LeanMqtt/Packets/VarHeader/Properties/Basic.lean
@@ -1,4 +1,4 @@
-import LeanMqtt.Primitives.Basic
+import LeanMqtt.Primitives.SizedList.Basic
 import LeanMqtt.Packets.VarHeader.Property.Basic
 import LeanMqtt.Packets.VarHeader.Property.Proofs
 
@@ -7,57 +7,12 @@ open Mqtt
 
 /- ========================= Properties ========================= -/
 
-abbrev Properties.rawByteSize (l : List Property) : Nat
-  := (l.map Property.byteSize).sum
-
-instance : GetByteSize (List Property) where
-  byteSize := Properties.rawByteSize
-
-abbrev Properties := WithByteSize (List Property) VarInt
+abbrev Properties := SizedList Property VarInt
 
 def Properties.serialize (ps : Properties) : List UInt8 :=
-  -- VarInt.serialize ps.len ++
-  -- ps.val.foldl (fun acc p => acc ++ p.serialize) []
-  VarInt.serialize ps.len ++ ps.val.flatMap Property.serialize
+  SizedList.serialize ps
 
-def parsePropsLoop (input : List UInt8) :
-  Option { ps : (List Property) // input.length = Properties.rawByteSize ps } :=
-  if h_empty : input.isEmpty then
-    some ⟨[], by
-      have h_len_zero : input.length = 0 := by grind
-      simp [h_len_zero, Properties.rawByteSize]
-    ⟩
-  else
-    match h_parse : Property.parser.run input with
-    | some (p, rest) =>
-      match parsePropsLoop rest with
-      | some ⟨tail, h_tail_len⟩ =>
-        let h_len_ps : input.length = Properties.rawByteSize (p :: tail) := by
-          have h_consumed : input.length = p.byteSize + rest.length
-            := Property.parser_len_consumed input p rest h_parse
-          rw [h_tail_len] at h_consumed
-          exact h_consumed
-
-        some ⟨(p :: tail), h_len_ps⟩
-      | none => none
-    | none => none
-termination_by input.length
-decreasing_by
-  have h_consumed := Property.parser_len_consumed input p rest h_parse
-  have h_pos := Property.byteSize_pos p
-  omega
-
-def Properties.parser : Parser Properties := do
-  let len ← VarInt.parser
-  let ⟨chunk, h_chunk_len⟩ ← bytesParserWithProof len
-
-  match parsePropsLoop chunk with
-  | some ⟨props, h_loop_len⟩ =>
-    have h_len : len.val = (props.map Property.byteSize).sum := by
-      rw [← h_chunk_len]
-      exact h_loop_len
-
-    return { val := props, len := ⟨len, h_len⟩ }
-  | none => none
+def Properties.parser : Parser Properties :=
+  SizedList.parser
 
 end Mqtt
