LeanMqtt/Core/Codec.lean
@@ -1,0 +1,14 @@
+import LeanMqtt.Core.Parser.Basic
+
+namespace Mqtt
+open Mqtt
+
+/--
+  A typeclass for basic, context-free types that can be serialized
+  and parsed without any external information.
+-/
+class Codec (α : Type) where
+  parser : Parser α
+  serialize : α → List UInt8
+  roundtrip : ∀ (a : α) (rest : List UInt8),
+    parser.run (serialize a ++ rest) = some (a, rest)
