LeanMqtt/Primitives/SizedList/Proofs.lean
@@ -1,0 +1,106 @@
+import LeanMqtt.Helpers.Proofs
+import LeanMqtt.Helpers.NatifyUInt8
+import LeanMqtt.Helpers.CrushLits
+
+import LeanMqtt.Core.Parser.Proofs
+import LeanMqtt.Primitives.Basic
+import LeanMqtt.Primitives.SizedList.Basic
+
+namespace Mqtt
+open Mqtt
+
+theorem ChunkItem.serialize_length {α : Type} [GetByteSize α] [ChunkItem α] (a : α) :
+  (ChunkItem.serialize a).length = GetByteSize.byteSize a := by
+  have h_rt := ChunkItem.roundtrip a []
+  have h_c := ChunkItem.h_consumed (ChunkItem.serialize a ++ []) a [] h_rt
+  simp at h_c
+  exact h_c
+
+theorem ChunkItem.serialize_list_length {α : Type}
+  [GetByteSize α] [ChunkItem α] (l : List α) :
+  (l.flatMap ChunkItem.serialize).length = List.rawByteSize l := by
+  induction l with
+  | nil => rfl
+  | cons a as ih =>
+    simp only [List.flatMap_cons, List.length_append]
+    rw [ChunkItem.serialize_length a]
+    rw [ih]
+    rfl
+
+theorem ChunkItem.serialize_not_empty {α : Type}
+  [GetByteSize α] [ChunkItem α] (a : α) (rest : List UInt8) :
+  (ChunkItem.serialize a ++ rest).isEmpty = false := by
+  cases h : ChunkItem.serialize a ++ rest with
+  | nil =>
+    have h_len : (ChunkItem.serialize a ++ rest).length = 0 := by rw [h]; rfl
+    have h_pos := ChunkItem.h_pos a
+    have h_a_len := ChunkItem.serialize_length a
+    rw [List.length_append, h_a_len] at h_len
+    omega
+  | cons _ _ => rfl
+
+theorem ChunkItem.parseChunkLoop_roundtrip {α : Type}
+  [s : GetByteSize α] [c : ChunkItem α] (l : List α) :
+  ∃ h, ChunkItem.parseChunkLoop (l.flatMap ChunkItem.serialize) = some ⟨l, h⟩ := by
+  induction l with
+  | nil =>
+    simp [List.flatMap_nil]
+    unfold ChunkItem.parseChunkLoop
+    simp
+  | cons a as ih =>
+    have h_input :
+        (a :: as).flatMap ChunkItem.serialize
+      = ChunkItem.serialize a ++ as.flatMap ChunkItem.serialize := rfl
+    rw [h_input]
+
+    unfold ChunkItem.parseChunkLoop
+
+    have h_not_empty := ChunkItem.serialize_not_empty a (as.flatMap ChunkItem.serialize)
+    simp [h_not_empty]
+
+    have h_rt := ChunkItem.roundtrip a (as.flatMap ChunkItem.serialize)
+
+    split
+    · next item rest h_parse_eq =>
+      rw [h_rt] at h_parse_eq
+
+      injection h_parse_eq with h_pair_eq
+      injection h_pair_eq with h_item h_rest
+
+      subst h_item
+      subst h_rest
+
+      obtain ⟨h_ih_proof, h_ih_eq⟩ := ih
+      rw [h_ih_eq]
+
+      exact ⟨by simp [ChunkItem.serialize_length], rfl⟩
+    · next h_parse_eq =>
+      rw [h_rt] at h_parse_eq
+      contradiction
+
+theorem SizedList.roundtrip {α lenTyp : Type}
+  [GetByteSize α] [Coe lenTyp Nat] [ChunkItem α] [Codec lenTyp]
+  (sl : SizedList α lenTyp) (rest : List UInt8) :
+  SizedList.parser.run (SizedList.serialize sl ++ rest) = some (sl, rest) := by
+
+  simp [SizedList.parser, SizedList.serialize, Option.bind]
+
+  rw [Codec.roundtrip sl.len.val _]
+  simp
+
+  have h_len_eq : (sl.len.val : Nat) = (sl.val.flatMap ChunkItem.serialize).length := by
+    rw [ChunkItem.serialize_list_length]
+    exact sl.len_eq
+
+  -- Bypass dependent type shenanigans on the byte parser
+  have h_simple := roundtrip_bytes (sl.val.flatMap ChunkItem.serialize) rest
+  rw [←h_len_eq] at h_simple
+  have ⟨_, h_dep⟩ := bytesParserWithProof_eq_parser_success _ _ _ _ h_simple
+
+  rw [h_dep]
+  simp
+
+  have ⟨h_loop_proof, h_loop_eq⟩ := ChunkItem.parseChunkLoop_roundtrip sl.val
+  rw [h_loop_eq]
+
+  simp
